src/traversal/TraversalProperties.v
@@ -1,0 +1,123 @@
+Require Import Classical Peano_dec Setoid PeanoNat.
+From hahn Require Import Hahn.
+
+Require Import Events.
+Require Import Execution.
+Require Import Execution_eco.
+Require Import imm_s_hb.
+Require Import imm_s.
+Require Import imm_bob imm_s_ppo.
+Require Import CombRelations.
+Require Import imm_s_rfppo.
+Require Import AuxDef.
+Require Import AuxRel2.
+Require Import TraversalConfig.
+Require Import Traversal.
+
+Section TraversalProperties.
+  Variable G : execution.
+  Variable WF : Wf G.
+  Variable sc : relation actid.
+  Variable IMMCON : imm_consistent G sc.
+
+  Notation "'acts'" := G.(acts).
+  Notation "'sb'" := G.(sb).
+  Notation "'rmw'" := G.(rmw).
+  Notation "'data'" := G.(data).
+  Notation "'addr'" := G.(addr).
+  Notation "'ctrl'" := G.(ctrl).
+  Notation "'rf'" := G.(rf).
+  Notation "'co'" := G.(co).
+  Notation "'coe'" := G.(coe).
+  Notation "'fr'" := G.(fr).
+
+  Notation "'eco'" := G.(eco).
+
+  Notation "'bob'" := G.(bob).
+  Notation "'fwbob'" := G.(fwbob).
+  Notation "'ppo'" := G.(ppo).
+  Notation "'fre'" := G.(fre).
+  Notation "'rfi'" := G.(rfi).
+  Notation "'rfe'" := G.(rfe).
+  Notation "'deps'" := G.(deps).
+  Notation "'detour'" := G.(detour).
+  Notation "'release'" := G.(release).
+  Notation "'sw'" := G.(sw).
+  Notation "'hb'" := G.(hb).
+
+  Notation "'urr'" := (urr G sc).
+  Notation "'c_acq'" := (c_acq G sc).
+  Notation "'c_cur'" := (c_cur G sc).
+  Notation "'c_rel'" := (c_rel G sc).
+  Notation "'t_acq'" := (t_acq G sc).
+  Notation "'t_cur'" := (t_cur G sc).
+  Notation "'t_rel'" := (t_rel G sc).
+  Notation "'S_tm'" := G.(S_tm).
+  Notation "'S_tmr'" := G.(S_tmr).
+  Notation "'msg_rel'" := (msg_rel G sc).
+
+Notation "'lab'" := G.(lab).
+Notation "'loc'" := (loc lab).
+Notation "'val'" := (val lab).
+Notation "'mod'" := (Events.mod lab).
+Notation "'same_loc'" := (same_loc lab).
+
+Notation "'E'" := G.(acts_set).
+Notation "'R'" := (fun x => is_true (is_r lab x)).
+Notation "'W'" := (fun x => is_true (is_w lab x)).
+Notation "'F'" := (fun x => is_true (is_f lab x)).
+Notation "'RW'" := (R ∪₁ W).
+Notation "'FR'" := (F ∪₁ R).
+Notation "'FW'" := (F ∪₁ W).
+
+Notation "'R_ex'" := (R_ex G).
+Notation "'W_ex'" := (W_ex G).
+Notation "'W_ex_acq'" := (W_ex ∩₁ (fun a => is_true (is_xacq lab a))).
+
+Notation "'Init'" := (fun a => is_true (is_init a)).
+Notation "'Loc_' l" := (fun x => loc x = Some l) (at level 1).
+Notation "'Tid_' t" := (fun x => tid x = t) (at level 1).
+Notation "'W_' l" := (W ∩₁ Loc_ l) (at level 1).
+
+Notation "'Pln'" := (fun x => is_true (is_only_pln lab x)).
+Notation "'Rlx'" := (fun x => is_true (is_rlx lab x)).
+Notation "'Rel'" := (fun x => is_true (is_rel lab x)).
+Notation "'Acq'" := (fun x => is_true (is_acq lab x)).
+Notation "'Acqrel'" := (fun x => is_true (is_acqrel lab x)).
+Notation "'Sc'" := (fun x => is_true (is_sc lab x)).
+Notation "'Acq/Rel'" := (fun a => is_true (is_ra lab a)).
+
+Variable T : trav_config.
+Hypothesis TCCOH : tc_coherent G sc T.
+
+Lemma itrav_stepE e T' (STEP : itrav_step G sc e T T') :
+  E e.
+Proof using TCCOH.
+  assert (tc_coherent G sc T') as TCCOH'.
+  { eapply trav_step_coherence; eauto. red. eauto. }
+  red in STEP. desf.
+  { eapply coveredE with (T:=T'); eauto. apply COVEQ. basic_solver. }
+  eapply issuedE with (T:=T'); eauto. apply ISSEQ. basic_solver.
+Qed.
+
+Lemma dom_rfrmw_issuable_in_I :
+  dom_rel (rf ⨾ rmw ⨾ ⦗issuable G sc T⦘) ⊆₁ issued T.
+Proof using WF TCCOH.
+  rewrite <- rfrmw_coverable_issuable_in_I; eauto.
+  basic_solver 10.
+Qed.
+
+Lemma I_rfrmw_issuable :
+  rf ⨾ rmw ⨾ ⦗issuable G sc T⦘ ≡ ⦗issued T⦘ ⨾ rf ⨾ rmw ⨾ ⦗issuable G sc T⦘.
+Proof using WF TCCOH. apply dom_rel_helper. by apply dom_rfrmw_issuable_in_I. Qed.
+
+Lemma issuable_W_ex_in_codom_I_rfrmw :
+  issuable G sc T ∩₁ W_ex ⊆₁ codom_rel (⦗issued T⦘ ⨾ rf ⨾ rmw).
+Proof using WF TCCOH IMMCON.
+  rewrite W_ex_in_codom_rfrmw; eauto.
+  rewrite set_interC. rewrite <- codom_eqv1, seqA.
+  rewrite I_rfrmw_issuable; auto.
+  basic_solver 10.
+Qed.
+
+End TraversalProperties.
